Mostly automated proof search with opburn.

src/Repr/SystemFOp/Kind.v
@@ -1,7 +1,7 @@
 Require Import List.
 Require Import Repr.Lists.
 
-Inductive kind : Type :=
+Inductive kind : Set :=
   | KStar : kind .
 
 Definition kenv := list kind.
