src/Repr/SystemFOp/Type.v
@@ -4,6 +4,7 @@ Require Import Repr.Lists.
 
 Require Import Repr.Tactics.
 Require Import Repr.Tactics.LibTactics.
+Require Import Repr.Tactics.Opburn.
 
 Require Import Coq.Arith.Peano_dec.
 Require Import Coq.Arith.Compare_dec.
@@ -38,8 +39,8 @@ Inductive well_formed_typ : kenv -> typ -> Prop :=
         well_formed_typ D T2 ->
         well_formed_typ D (TArrow T1 T2)
   | WFT_TAll :
-      forall D K T,
-        well_formed_typ (K :: D) T ->
+      forall D T,
+        (exists K, well_formed_typ (K :: D) T) ->
         well_formed_typ D (TAll T) .
 
 Hint Constructors well_formed_typ.
@@ -140,95 +141,114 @@ Ltac case_lift :=
       case (lift_le_gt_dec a b)
   end.
 
+(* Mega tactic that deals with all the de bruijn comparisons *)
 Ltac burn_tvar :=
   simpl;
   match goal with
     | [ |- context[nat_compare _ _ ] ]
       => break_nat_compare ;
-         tburn;
+         opburn ;
          burn_tvar
+    | [ |- context[ match nat_compare ?n ?m with 
+                      | Eq => _ 
+                      | Lt => _ 
+                      | Gt => _  
+                    end ] ]
+      => break (nat_compare n m) ;
+         norm_nat_compare ;
+         opburn ;
+         burn_tvar 
     | [ |- context [lift_le_gt_dec _ _ ] ]
       => case_lift ;
-         tburn;
+         opburn ;
          burn_tvar
+     | [ |- context [ match ?n with O => _ | S _ => _ end ] ] 
+       => destruct n ;
+          opburn ;
+          burn_tvar
     | _ 
-      => tburn
+      => opburn
   end.
 
 Lemma typ_subs_nil_typ_lift
   :  forall X U T
   ,  [X |=> U] (typ_lift X T) = T.
 Proof.
-  rip; gen X U; induction_kind T; destruct X; burn_tvar.
+  linduction T; destruct X; opburn' tt tt kind_rel; burn_tvar.
 Qed.
-Hint Rewrite typ_subs_nil_typ_lift.
-
-Lemma tall_injective 
-  :  forall (T1 T2:typ)
-  ,  T1 = T2
-  -> TAll T1 = TAll T2.
-Proof. burn. Qed.
 
 Lemma typ_lift_SX
   :  forall (X Y:tvar)(T:typ)
   ,  Y <= X
   -> typ_lift (S X) (typ_lift Y T) = typ_lift Y (typ_lift X T).
 Proof.
-  rip; gen X Y; induction T; tburn; rip; burn_tvar.
-Qed.  
+  linduction T; opburn' tt tt kind_rel; burn_tvar.
+Qed.
+
+Definition marker_Snm (n n':nat) := S n + n'.
+Hint Unfold marker_Snm.
+
+Lemma Snm_Snpm 
+  :  forall (n m : nat)
+  ,  S (n + m) = marker_Snm n m.
+Proof. opburn. Qed.
 
 Lemma typ_lift_over_subs
   :  forall (n n':nat)(U T:typ)
   ,  typ_lift n ([(n + n') |=> U] T) 
   =  [(1 + n + n') |=> typ_lift n U] typ_lift n T.
 Proof.
-  rip; gen n n' U; induction T; tburn.
-  rip; burn_tvar.
-
-  rip; simpl; eapply tall_injective.
-  assert (S (n + n') = S n + n'). burn. rewrite H. rewrite IHT. simpl.
-
-  rewrite typ_lift_SX; burn. 
+  linduction T; 
+  opburn' 
+    tt 
+    (typ_lift_SX, Snm_Snpm) 
+    kind_rel; 
+  [burn_tvar].
 Qed.
-Hint Rewrite typ_lift_over_subs.
 
 Lemma typ_lift_over_subs'
   :  forall (n n':nat)(U T:typ)
   ,  typ_lift (n + n') ([n |=> U] T) 
   =  [n  |=> typ_lift (n + n') U] typ_lift (1 + n + n') T.
 Proof.
-  rip; gen n n' U; induction T; tburn.
-  
-  rip; destruct n; burn_tvar.
-
-  rip. simpl. eapply tall_injective. 
-  assert (S (n + n') = S n + n'). burn. rewrite H. rewrite IHT. simpl.
-  rewrite typ_lift_SX; burn.
+  linduction T;
+  opburn'
+    tt
+    (typ_lift_SX, Snm_Snpm)
+    kind_rel;
+  [burn_tvar].
 Qed.
-Hint Rewrite typ_lift_over_subs.
 
-(* LAST : Solve *)
+Definition marker_Onm (n n':nat) := O + (n + n').
+Hint Unfold marker_Onm.
+
+Lemma Onm 
+  :  forall (n m : nat)
+  ,  (n + m) = marker_Onm n m.
+Proof. opburn. Qed.
+
+Lemma Onm_ONCE : rewrite_ONCE (Onm).
+  constructor.
+Qed.
+
+(* LAST *)
+(* Coq tuples are right associative, we need our own notation *)
+
+
 
 Lemma commute_typ_subs
   :  forall (n n':nat)(T1 T2 T3:typ)
   ,  [n + n' |=> T3] ([n |=> T2] T1)
   =  [n |=> [ n + n' |=> T3] T2 ] ([1 + n + n' |=> (typ_lift n T3)] T1).
 Proof.
-  rip; gen n n' T2 T3 ; induction_kind T1.
-  burn_tvar.
-  break (nat_compare n (S (n + n'))); norm_nat_compare; simpl; tburn.
-  burn_tvar.
-  
-  eapply tall_injective.
-  assert (n + n' = 0 + (n + n')) by burn. rewrite H at 2.
-  rewrite typ_lift_over_subs; simpl.
-  
-  assert (S (n + n') = S n + n') by burn. rewrite H0.
-  assert (S (S n + n') = 1 + S n + n') by burn. rewrite H1.
-  rewrite IHT1.
-  rewrite typ_lift_SX; burn.
+  linduction T1; 
+  opburn' 
+    tt 
+    (Onm_ONCE, Snm_Snpm, typ_lift_SX, typ_lift_over_subs)
+    kind_rel;
+  [burn_tvar];
+  opburn' tt typ_subs_nil_typ_lift tt.
 Qed.
-
 
 (********************************************************************)
 
@@ -238,46 +258,46 @@ Lemma kind_rel_imp_well_formed_typ
   ,  D \\- T \: K
   -> well_formed_typ D T.
 Proof.
-  rip; gen D K; induction_kind T.
+  linduction T; opburn' tt tt kind_rel; eauto.
 Qed.
-Hint Resolve kind_rel_imp_well_formed_typ.
 
-(* We may insert into a kind environment at X provided we lift all
- * types that occuring after X in the kind environment. 
- *
- * NOTE: This attempt at automation shows where the burn tactic fails,
- * and one area where crush does well. Specifically, burn doesn't do
- * a great job with rewriting after constructors are needed.
- *
- * It is tricky --- If you rewrite too soon or too late you will block
- * the resolution process. Something I want to return to and study. *)
+(* NOTE: inster will fall on polymorphic types, but we can make it work
+   by trying to *type of* all H's on the goal. *)
+(* One dirty trick due to K's rewrite *)
 Lemma kind_rel_insert
   :  forall D T K X
   ,  D \\- T \: K
   -> insert D X KStar \\- typ_lift X T \: K.
 Proof.
-  Hint Rewrite insert_rewind.
-  rip; gen D K X; induction_kind T;
+  linduction T; 
+  opburn'' 
+    tt 
+    insert_rewind 
+    kind_rel 
+    ltac:(fun H => match type of H with | kind => rewrite H in * end);
   match goal with
     (* TVar *)
     | [ |- context [lift_le_gt_dec ?A ?B] ] 
-      => break (lift_le_gt_dec A B); tburn
+      => break (lift_le_gt_dec A B) ;
+           econstructor ;
+           opburn' (get_insert_above_idx' kind) get_insert_below_idx tt
     (* TAbs *)
     | _ 
-      => econstructor; autorewrite_goal; burn
+      => econstructor; opburn' tt insert_rewind kind_rel_insert
   end.
-  Remove Hints insert_rewind.
 Qed.
-Hint Resolve kind_rel_insert.
 
 Theorem kind_rel_weakening
   :  forall D T K
   ,  D \\- T \: K
   -> (KStar :: D) \\- typ_lift 0 T \: K.
 Proof.
-  rip; rewrite cons_as_insert; burn.
+  intros; rewrite K in *;
+  opburn' 
+    kind_rel_insert 
+    cons_as_insert 
+    tt.    
 Qed.  
-Hint Resolve kind_rel_weakening.
 
 Lemma type_substition_preserves_kinding'
   :  forall (D:kenv)(X:tvar)(U T:typ)
@@ -285,19 +305,31 @@ Lemma type_substition_preserves_kinding'
   -> D \\- T \: KStar
   -> delete D X \\- [X |=> U] T \: KStar.
 Proof.
-  rip; gen D X U; induction_kind T.
-  burn_tvar. econstructor. burn.
-  econstructor; rewrite delete_rewind; eapply IHT; burn.
+  linduction T; 
+  opburn' 
+    kind_rel_weakening
+    delete_rewind
+    kind_rel;
+  [ (* T-Var *)
+    burn_tvar; econstructor ;
+    opburn' tt (get_delete_above_idx, get_delete_below_idx) tt
+  | (* T-All *)
+    econstructor ;
+    match goal with
+    | [ H : delete ?D ?X \\- _ \: _ |- _ ] =>
+      let x := fresh "D" in
+      pose (x := delete D X)
+    end ;
+    opburn' kind_rel_weakening delete_rewind tt 
+  ].
 Qed.
-Hint Resolve type_substition_preserves_kinding'.
 
 Lemma type_substition_preserves_kinding
   :  forall (D:kenv)(X:tvar)(U T:typ)
   ,  delete (KStar :: D) 0 \\- U \: KStar
   -> (KStar :: D) \\- T \: KStar
   -> delete (KStar :: D) 0 \\- [0 |=> U] T \: KStar.
-Proof. rip; burn. Qed.
-
+Proof. intros; eapply type_substition_preserves_kinding'; opburn. Qed.
 
 (********************************************************************)
 
@@ -309,11 +341,9 @@ Hint Unfold tenv.
  * new type variables are 'pushed' *)
 Definition tenv_lift (dp:nat)(G:tenv) : tenv := 
   map (typ_lift dp) G.
-Hint Unfold tenv_lift.
 
 Definition tenv_substitute (X:tvar)(U:typ)(G:tenv) : tenv := 
   map (typ_substitute X U) G.
-Hint Unfold tenv_substitute.
 
 (********************************************************************)
 
@@ -321,7 +351,7 @@ Lemma delete_tenv_lift
   :  forall G x
   ,  delete (tenv_lift 0 G) x = tenv_lift 0 (delete G x).
 Proof.
-  rip; gen G; induction x; destruct G; tburn.
+  linduction x; destruct G; opburn.
 Qed.
 
 Lemma get_tenv_lift
@@ -329,23 +359,19 @@ Lemma get_tenv_lift
   ,  get G x = Some T
   -> get (tenv_lift X G) x = Some (typ_lift X T).
 Proof.
-  induction G; destruct x; rip; 
-  simpl in *; try norm_some; tburn.
+  linduction G; destruct x; opburn.
 Qed.
-Hint Resolve get_tenv_lift.
 
 Lemma rewind_tenv_lift
   :  forall G T X
   ,  typ_lift X T :: tenv_lift X G = tenv_lift X (T :: G).
-Proof. burn. Qed.
-Hint Rewrite rewind_tenv_lift.
+Proof. opburn. Qed.
 
 Lemma tenv_lift_SX
   :  forall G X
   ,  tenv_lift 0 (tenv_lift X G) = tenv_lift (S X) (tenv_lift 0 G).
 Proof.
-  induction G; rip; simpl; tburn.
-  rewrite IHG; rewrite typ_lift_SX; burn.
+  linduction G; opburn' tt typ_lift_SX tt.
 Qed.
 
 Lemma get_tenv_substitute
@@ -353,36 +379,34 @@ Lemma get_tenv_substitute
   ,  get G Y = Some T
   -> get (tenv_substitute X U G) Y = Some ([X |=> U] T).
 Proof.  
-  induction G; destruct Y; rip;
-  simpl in *; try norm_some; tburn.
+  linduction G; destruct Y; opburn.
 Qed.
-Hint Resolve get_tenv_substitute.
 
 Lemma rewind_tenv_substitute
   :  forall G U T X
   ,  [X |=> U] T :: tenv_substitute X U G = tenv_substitute X U (T :: G).
-Proof. burn. Qed.
-Hint Rewrite rewind_tenv_substitute.
+Proof. opburn. Qed.
 
 Lemma typ_lift_over_tenv_subs
   :  forall (n n':nat)(U:typ)(D:tenv)
   ,  tenv_lift n (tenv_substitute (n + n') U D) 
   =  tenv_substitute (1 + n + n') (typ_lift n U) (tenv_lift n D).
 Proof.
-  rip; gen n n' U; induction D; tburn.
-  rip. simpl. rewrite IHD. simpl.
-  burn.
+  linduction D; 
+  opburn' 
+    tt 
+    (typ_lift_over_subs, rewind_tenv_substitute, rewind_tenv_lift)
+    tt.
 Qed.
-Hint Rewrite typ_lift_over_tenv_subs.
 
 Lemma typ_lift_over_tenv_subs'
   :  forall (n n':nat)(U:typ)(D:tenv)
   ,  tenv_lift (n + n') (tenv_substitute n U D) 
   =  tenv_substitute n (typ_lift (n + n') U) (tenv_lift (1 + n + n') D).
 Proof.
-  rip; gen n n' U; induction D; tburn.
-  rip. simpl. rewrite IHD. simpl. 
-  rewrite typ_lift_over_subs'. burn.
+  linduction D; 
+  opburn' 
+    tt 
+    (typ_lift_over_subs', rewind_tenv_substitute, rewind_tenv_lift)
+    tt.
 Qed.
-Hint Rewrite typ_lift_over_tenv_subs'.
-
